thys/LLL_Basis_Reduction/LLL_Mu_Integer_Impl.thy
@@ -1,0 +1,926 @@
+(*
+    Authors:    René Thiemann
+    License:    BSD
+*)
+subsection \<open>LLL Implementation which Stores Multiples of the $\mu$-values and the Norms of the GSO as Integers\<close>
+
+theory LLL_Mu_Integer_Impl
+  imports LLL
+   List_Representation
+   LLL_Number_Bounds
+begin
+
+text \<open>We store the $f$, $\mu$, and $||g||^2$ values.\<close>
+
+definition iarray_update :: "'a iarray \<Rightarrow> nat \<Rightarrow> 'a \<Rightarrow> 'a iarray" where
+  "iarray_update a i x = IArray.of_fun (\<lambda> j. if j = i then x else IArray.sub a j) (IArray.length a)" 
+
+lemma iarray_of_fun_cong: "(\<And> i. i < n \<Longrightarrow> f i = g i) \<Longrightarrow> IArray.of_fun f n = IArray.of_fun g n" 
+  unfolding IArray.of_fun_def by auto
+
+lemma iarray_length_of_fun[simp]: "IArray.length (IArray.of_fun f n) = n" by simp
+
+lemma division_to_div: "rat_of_int x = of_int y / of_int z \<Longrightarrow> x = y div z" 
+  by (metis floor_divide_of_int_eq floor_of_int)
+
+hide_fact Word.inc_i
+
+type_synonym LLL_gso_state = "int vec list_repr \<times> int iarray iarray \<times> int iarray"
+
+fun fi_state :: "LLL_gso_state \<Rightarrow> int vec" where
+  "fi_state (f,mu,d) = get_nth_i f" 
+
+fun fim1_state :: "LLL_gso_state \<Rightarrow> int vec" where
+  "fim1_state (f,mu,d) = get_nth_im1 f" 
+
+fun d_state :: "LLL_gso_state \<Rightarrow> nat \<Rightarrow> int" where
+  "d_state (f,mu,d) i = IArray.sub d i" 
+
+fun fs_state :: "LLL_gso_state \<Rightarrow> int vec list" where
+  "fs_state (f,mu,d) = of_list_repr f" 
+
+fun upd_fi_mu_state :: "LLL_gso_state \<Rightarrow> nat \<Rightarrow> int vec \<Rightarrow> int iarray \<Rightarrow> LLL_gso_state" where
+  "upd_fi_mu_state (f,mu,d) i fi mu_i = (update_i f fi, iarray_update mu i mu_i,d)" 
+
+fun small_fs_state :: "LLL_gso_state \<Rightarrow> int vec list" where
+  "small_fs_state (f,_) = fst f" 
+
+fun dmu_ij_state :: "LLL_gso_state \<Rightarrow> nat \<Rightarrow> nat \<Rightarrow> int" where
+  "dmu_ij_state (f,mu,_) i j = IArray.sub (IArray.sub mu i) j" 
+
+fun inc_state :: "LLL_gso_state \<Rightarrow> LLL_gso_state" where
+  "inc_state (f,mu,d) = (inc_i f, mu, d)" 
+
+definition floor_ceil_num_denom :: "int \<Rightarrow> int \<Rightarrow> int" where
+  "floor_ceil_num_denom n d = ((2 * n + d) div (2 * d))" 
+
+lemma floor_ceil_num_denom: "denom > 0 \<Longrightarrow> floor_ceil_num_denom num denom = 
+  floor_ceil (of_int num / rat_of_int denom)" 
+  unfolding floor_ceil_def floor_ceil_num_denom_def
+  unfolding floor_divide_of_int_eq[where ?'a = rat, symmetric]
+  by (rule arg_cong[of _ _ floor], simp add: add_divide_distrib)
+
+fun basis_reduction_add_rows_loop where
+  "basis_reduction_add_rows_loop state i j [] = state" 
+| "basis_reduction_add_rows_loop state i sj (fj # fjs) = (
+     let fi = fi_state state;
+         dsj = d_state state sj;
+         j = sj - 1;
+         c = floor_ceil_num_denom (dmu_ij_state state i j) dsj;
+         state' = (if c = 0 then state else upd_fi_mu_state state i (fi - c \<cdot>\<^sub>v fj) 
+             (IArray.of_fun (\<lambda> jj. let mu = dmu_ij_state state i jj in 
+                  if jj < j then mu - c * dmu_ij_state state j jj else 
+                  if jj = j then mu - dsj * c else mu) i))
+      in basis_reduction_add_rows_loop state' i j fjs)"
+
+text \<open>More efficient code which breaks abstraction of state.\<close>
+
+lemma basis_reduction_add_rows_loop_code: 
+  "basis_reduction_add_rows_loop state i sj (fj # fjs) = (
+     case state of ((f1,f2),mus,ds) \<Rightarrow> 
+     let fi = hd f2;
+         j = sj - 1;
+         dsj = IArray.sub ds sj;
+         mui = IArray.sub (IArray.sub mus i);
+         c = floor_ceil_num_denom (mui j) dsj
+      in (if c = 0 then 
+          basis_reduction_add_rows_loop state i j fjs
+         else  
+             let muj = IArray.sub (IArray.sub mus j) in 
+           basis_reduction_add_rows_loop
+                ((f1,  (fi - c \<cdot>\<^sub>v fj) # tl f2), iarray_update mus i 
+             (IArray.of_fun (\<lambda> jj. let mu = mui jj in 
+                  if jj < j then mu - c * muj jj else 
+                  if jj = j then mu - dsj * c else mu) i),
+                  ds) i j fjs))"
+proof -
+  obtain f1 f2 mus ds where state: "state = ((f1,f2),mus, ds)" by (cases state, auto)
+  show ?thesis unfolding basis_reduction_add_rows_loop.simps Let_def 
+     state split dmu_ij_state.simps fi_state.simps get_nth_i_def update_i_def upd_fi_mu_state.simps
+     d_state.simps
+    by simp
+qed
+
+lemmas basis_reduction_add_rows_loop_code_equations =
+  basis_reduction_add_rows_loop.simps(1) basis_reduction_add_rows_loop_code
+
+declare basis_reduction_add_rows_loop_code_equations[code]
+
+
+definition basis_reduction_add_rows where
+  "basis_reduction_add_rows upw i state = 
+     (if upw 
+        then basis_reduction_add_rows_loop state i i (small_fs_state state) 
+        else state)" 
+
+context
+  fixes \<alpha> :: rat and n m :: nat and fs_init :: "int vec list" 
+begin
+
+definition swap_mu :: "int iarray iarray \<Rightarrow> nat \<Rightarrow> int \<Rightarrow> int \<Rightarrow> int \<Rightarrow> int \<Rightarrow> int iarray iarray" where
+  "swap_mu dmu i dmu_i_im1 dim1 di dsi = (let im1 = i - 1 in 
+       IArray.of_fun (\<lambda> ii. if ii < im1 then IArray.sub dmu ii else 
+       if ii > i then let dmu_ii = IArray.sub (IArray.sub dmu ii) in 
+           IArray.of_fun (\<lambda> j. let dmu_ii_j = dmu_ii j in 
+               if j = i then (dsi * dmu_ii im1 - dmu_i_im1 * dmu_ii i) div di
+               else if j = im1 then (dmu_i_im1 * dmu_ii j + dmu_ii i * dim1) div di
+               else dmu_ii_j) ii else 
+       if ii = i then let mu_im1 = IArray.sub (IArray.sub dmu im1) in 
+           IArray.of_fun (\<lambda> j. if j = im1 then dmu_i_im1 else mu_im1 j) ii 
+         else IArray.of_fun (IArray.sub (IArray.sub dmu i)) ii) \<comment> \<open>ii = i - 1\<close>
+       m)" 
+
+definition basis_reduction_swap where
+  "basis_reduction_swap i state = (let 
+       di = d_state state i;
+       dsi = d_state state (Suc i);
+       dim1 = d_state state (i - 1);
+       fi = fi_state state;
+       fim1 = fim1_state state;
+       dmu_i_im1 = dmu_ij_state state i (i - 1);
+       fi' = fim1;
+       fim1' = fi
+     in (case state of (f,dmus,djs) \<Rightarrow>
+         (False, i - 1, 
+           (dec_i (update_im1 (update_i f fi') fim1'), 
+            swap_mu dmus i dmu_i_im1 dim1 di dsi, 
+            iarray_update djs i ((dsi * dim1 + dmu_i_im1 * dmu_i_im1) div di)))))"
+
+text \<open>More efficient code which breaks abstraction of state.\<close>
+
+lemma basis_reduction_swap_code[code]:
+  "basis_reduction_swap i ((f1,f2), dmus, ds) = (let 
+       di = IArray.sub ds i;
+       dsi = IArray.sub ds (Suc i);
+       im1 = i - 1;
+       dim1 = IArray.sub ds im1;
+       fi = hd f2;
+       fim1 = hd f1;
+       dmu_i_im1 = IArray.sub (IArray.sub dmus i) im1;
+       fi' = fim1;
+       fim1' = fi
+     in (False, im1, 
+           ((tl f1,fim1' # fi' # tl f2), 
+            swap_mu dmus i dmu_i_im1 dim1 di dsi, 
+            iarray_update ds i ((dsi * dim1 + dmu_i_im1 * dmu_i_im1) div di))))"
+proof - 
+  show ?thesis unfolding basis_reduction_swap_def split Let_def fi_state.simps fim1_state.simps 
+    d_state.simps get_nth_im1_def get_nth_i_def update_i_def update_im1_def dec_i_def
+    by simp
+qed
+
+definition basis_reduction_step where
+  "basis_reduction_step upw i state = (if i = 0 then (True, Suc i, inc_state state)
+     else let 
+       state' = basis_reduction_add_rows upw i state;
+       di = d_state state' i;
+       dsi = d_state state' (Suc i);
+       dim1 = d_state state' (i - 1);
+       (num,denom) = quotient_of \<alpha>
+    in if di * di * denom \<le> num * dim1 * dsi then
+          (True, Suc i, inc_state state') 
+        else basis_reduction_swap i state')" 
+
+partial_function (tailrec) basis_reduction_main where
+  [code]: "basis_reduction_main upw i state = (if i < m
+     then case basis_reduction_step upw i state of (upw',i',state') \<Rightarrow> 
+       basis_reduction_main upw' i' state' else
+       state)"
+
+fun norms_to_ds where 
+    "norms_to_ds d [] = [d]" 
+  | "norms_to_ds d (ni # nis) = (d # norms_to_ds (int_of_rat (int_times_rat d ni)) nis)" 
+
+(* TODO: use better gram_schmidt, which already computes mu-values *)
+definition "initial_state = (let
+  (n_gs, mus) = norms_mus_rat n (map (map_vec rat_of_int) fs_init);
+  ds = (IArray (norms_to_ds 1 n_gs) :: int iarray)
+  in (([], fs_init), 
+    IArray.of_fun (\<lambda> i. IArray.of_fun (\<lambda> j. int_of_rat (int_times_rat (IArray.sub ds (Suc j)) (mus ! i ! j))) i) m, 
+    ds) :: LLL_gso_state)" 
+
+end
+
+definition "basis_reduction \<alpha> n fs = basis_reduction_main \<alpha> (length fs) True 0 (initial_state n (length fs) fs)" 
+
+definition "reduce_basis \<alpha> fs = (case fs of Nil \<Rightarrow> fs | Cons f _ \<Rightarrow> fs_state (basis_reduction \<alpha> (dim_vec f) fs))" 
+
+definition "short_vector \<alpha> fs = hd (reduce_basis \<alpha> fs)"
+
+lemma map_rev_Suc: "map f (rev [0..<Suc j]) = f j # map f (rev [0..< j])" by simp
+
+context LLL
+begin
+
+definition mu_repr :: "int iarray iarray \<Rightarrow> int vec list \<Rightarrow> bool" where
+  "mu_repr mu fs = (mu = IArray.of_fun (\<lambda> i. IArray.of_fun (\<lambda> j. int_of_rat (of_int (d fs (Suc j)) * \<mu> fs i j)) i) m)" 
+
+definition d_repr :: "int iarray \<Rightarrow> int vec list \<Rightarrow> bool" where
+  "d_repr ds fs = (ds = IArray.of_fun (d fs) (Suc m))" 
+
+fun LLL_impl_inv :: "LLL_gso_state \<Rightarrow> nat \<Rightarrow> int vec list \<Rightarrow> bool" where
+  "LLL_impl_inv (f,mu,ds) i fs = (list_repr i f (map (\<lambda> j. fs ! j) [0..<m])
+    \<and> d_repr ds fs
+    \<and> mu_repr mu fs)" 
+
+context fixes state i fs upw f mu ds
+  assumes impl: "LLL_impl_inv state i fs"
+  and inv: "LLL_invariant upw i fs" 
+  and state: "state = (f,mu,ds)" 
+begin
+lemma to_list_repr: "list_repr i f (map ((!) fs) [0..<m])"
+  using impl[unfolded state] by auto
+
+lemma to_mu_repr: "mu_repr mu fs" using impl[unfolded state] by auto
+lemma to_d_repr: "d_repr ds fs" using impl[unfolded state] by auto
+
+lemma dmu_ij_state: assumes j: "j < ii" 
+  and ii: "ii < m" 
+shows "of_int (dmu_ij_state state ii j) = of_int (d fs (Suc j)) * \<mu> fs ii j" 
+  unfolding to_mu_repr[unfolded mu_repr_def] state using j ii
+  using LLL_mu_d_Z[OF inv j ii]
+  by auto
+
+lemma fi_state: "i < m \<Longrightarrow> fi_state state = fs ! i"
+  using get_nth_i[OF to_list_repr(1)] unfolding state by auto
+
+lemma fim1_state: "i < m \<Longrightarrow> i \<noteq> 0 \<Longrightarrow> fim1_state state = fs ! (i - 1)"
+  using get_nth_im1[OF to_list_repr(1)] unfolding state by auto
+
+lemma d_state: "ii \<le> m \<Longrightarrow> d_state state ii = d fs ii"
+  using to_d_repr[unfolded d_repr_def] state 
+  unfolding state by (auto simp: nth_append)
+
+lemma fs_state: "length fs = m \<Longrightarrow> fs_state state = fs"
+  using of_list_repr[OF to_list_repr(1)] unfolding state by (auto simp: o_def intro!: nth_equalityI)
+
+lemma LLL_state_inc_state: assumes i: "i < m"
+shows "LLL_impl_inv (inc_state state) (Suc i) fs" 
+  "fs_state (inc_state state) = fs_state state" 
+proof -
+  from LLL_invD[OF inv] have len: "length fs = m" by auto
+  note inc = inc_i[OF to_list_repr(1)] 
+  from inc i impl show "LLL_impl_inv (inc_state state) (Suc i) fs" 
+    unfolding state by auto
+  from of_list_repr[OF inc(1)] of_list_repr[OF to_list_repr(1)] i
+  show "fs_state (inc_state state) = fs_state state" unfolding state by auto
+qed
+end
+end
+
+lemma int_via_rat_eqI: "rat_of_int x = rat_of_int y \<Longrightarrow> x = y" by auto
+
+context LLL_with_assms
+begin
+lemma basis_reduction_add_rows_loop: assumes
+    impl: "LLL_impl_inv state i fs" 
+  and inv: "LLL_invariant True i fs" 
+  and mu_small: "\<mu>_small_row i fs j"
+  and res: "basis_reduction_add_rows_loop state i j 
+    (map ((!) fs) (rev [0 ..< j])) = state'" 
+    (is "basis_reduction_add_rows_loop state i j (?mapf fs j) = _")
+  and j: "j \<le> i" 
+  and i: "i < m" 
+  and fs': "fs' = fs_state state'" 
+shows 
+  "LLL_impl_inv state' i fs'" 
+  "LLL_invariant False i fs'" 
+  "LLL_measure i fs' = LLL_measure i fs" 
+proof (atomize(full), insert assms(1-6), induct j arbitrary: fs state)
+  case (0 fs state)
+  from LLL_invD[OF 0(2)] have len: "length fs = m" by auto
+  from fs_state[OF 0(1-2) _ len] have "fs_state state = fs" by (cases state, auto)
+  thus ?case using 0 basis_reduction_add_row_done[of i fs] i fs' by auto
+next
+  case (Suc j fs state)
+  hence j: "j < i" and id: "(j < i) = True" by auto
+  obtain f mu ds where state: "state = (f,mu,ds)" by (cases state, auto)
+  note Linv = Suc(3)
+  note inv = LLL_invD[OF Linv]
+  note impl = Suc(2)
+  from fi_state[OF impl Linv state i] have fi: "fi_state state = fs ! i" by auto
+  have id: "Suc j - 1 = j" by simp
+  note mu = dmu_ij_state[OF impl Linv state j i]
+  let ?c = "floor_ceil (\<mu> fs i j)" 
+  from LLL_d_pos[OF Linv] j i have dj: "d fs (Suc j) > 0" by auto
+  have fl_ceil: "floor_ceil_num_denom (dmu_ij_state state i j) (d fs (Suc j)) = ?c" 
+    by (subst floor_ceil_num_denom, unfold mu, insert dj, auto)
+  note d_state = d_state[OF impl Linv state]
+  from d_state[of "Suc j"] j i have djs: "d_state state (Suc j) = d fs (Suc j)" by auto
+  note res = Suc(5)[unfolded fl_ceil map_rev_Suc djs append.simps basis_reduction_add_rows_loop.simps fi Let_def mu id int_times_rat_def]
+  show ?case
+  proof (cases "?c = 0")
+    case True
+    from res[unfolded True] 
+    have res: "basis_reduction_add_rows_loop state i j (?mapf fs j) = state'" 
+      by simp
+    note step = Linv basis_reduction_add_row_main_0[OF Linv i j True Suc(4)]
+    show ?thesis using Suc(1)[OF impl step(1-2) res _ i] j by auto
+  next
+    case False
+    hence id: "(?c = 0) = False" by auto
+    define fi' where "fi' = fs ! i - ?c \<cdot>\<^sub>v fs ! j" 
+    obtain fs'' where fs'': "fs[i := fs ! i - ?c \<cdot>\<^sub>v fs ! j] = fs''" by auto
+    note step = basis_reduction_add_row_main[OF Linv i j refl refl Suc(4), unfolded fs'']
+    have map_id_f: "?mapf fs j = ?mapf fs'' j"  
+      by (rule nth_equalityI, insert j step(4) i, auto simp: rev_nth fs''[symmetric])
+    have nth_id: "[0..<m] ! i = i" using i by auto
+    note res = res[unfolded False map_id_f id if_False]
+    have fi: "fi' = fs'' ! i" unfolding fs''[symmetric] fi'_def using inv(7) i by auto
+    let ?fn = "\<lambda> fs i. (fs ! i, sq_norm (gso fs i))" 
+    have repr_id: "(map (?fn fs) [0..<m] [i := (fs'' ! i, \<parallel>gso fs'' i\<parallel>\<^sup>2)])
+      = (map (?fn fs'') [0..<m])" (is "?xs = ?ys") 
+    proof (rule nth_equalityI, force, intro allI impI)
+      fix j
+      assume "j < length ?xs" 
+      thus "?xs ! j = ?ys ! j" 
+        using step(4) unfolding fs''[symmetric] i 
+        by (cases "j = i", auto)
+    qed
+    let ?norm = "\<lambda> fs i. int_of_rat (of_int (d fs i * d fs i) * sq_norm (gso fs i))" 
+    let ?d = "\<lambda> fs i. d fs (Suc i)" 
+    let ?mu = "\<lambda>fs i j. int_of_rat (rat_of_int (d fs (Suc j)) * \<mu> fs i j)" 
+
+    let ?mu' = "IArray.of_fun
+       (\<lambda>jj. if jj < j then dmu_ij_state state i jj - ?c * dmu_ij_state state j jj
+             else if jj = j then dmu_ij_state state i jj - ?d fs j * ?c else dmu_ij_state state i jj) i" 
+    have mu': "?mu' = IArray.of_fun (?mu fs'' i) i" (is "_ = ?mu'i")
+    proof (rule iarray_of_fun_cong, goal_cases)
+      case (1 jj)
+      let ?muu = "of_int (d fs'' (Suc jj)) * \<mu> fs'' i jj" 
+      from 1 j i have jj: "jj \<le> i" and jm: "j < m" and jjm: "jj < m" by auto
+      have id: "rat_of_int (int_of_rat ?muu) = ?muu" 
+        using LLL_mu_d_Z[OF step(1) 1 i] by simp
+      have id': "d fs'' (Suc jj) = d fs (Suc jj)" by (rule step(6), insert jjm, auto)
+      define c where "c = ?c" 
+      show ?case 
+        by (rule int_via_rat_eqI, unfold if_distrib[of rat_of_int] of_int_diff of_int_mult
+        dmu_ij_state[OF impl Linv state 1 i] id, unfold id' step(5)[OF i jjm] c_def[symmetric],
+        unfold if_distrib[of "( * ) (rat_of_int (d fs (Suc jj)))"] ring_distribs,
+          insert dmu_ij_state[OF impl Linv state _ jm], auto simp: gs.\<mu>.simps)
+    qed
+    have d': "(map (?d fs) (rev [0..<j])) = (map (?d fs'') (rev [0..<j]))" 
+      by (rule nth_equalityI, force, intro allI impI, simp, subst step(6), insert j i, auto
+        simp: nth_rev)
+    have repr_id:
+      "map ((!) fs) [0..<m][i := (fs'' ! i)] = map ((!) fs'') [0..<m]" (is "?xs = ?ys")
+    proof (rule nth_equalityI, force, intro allI impI)
+      fix j
+      assume "j < length ?xs" 
+      thus "?xs ! j = ?ys ! j" unfolding fs''[symmetric] i by (cases "j = i", auto)
+    qed
+    have repr_id_d: 
+      "map (d fs) [0..<Suc m] = map (d fs'') [0..<Suc m]"
+      by (rule nth_equalityI, force, intro allI impI, insert step(4,6), auto simp: nth_append)
+    have mu: "fs ! i - ?c \<cdot>\<^sub>v fs ! j = fs'' ! i" unfolding fs''[symmetric] using inv(7) i by auto
+    note res = res[unfolded mu' mu d']
+    show ?thesis unfolding step(3)[symmetric]
+    proof (rule Suc(1)[OF _ step(1,2) res _ i])
+      note list_repr = to_list_repr[OF impl Linv state]
+      from i have ii: "i < length [0..<m]" by auto
+      show "LLL_impl_inv (upd_fi_mu_state state i (fs'' ! i) ?mu'i) i fs''" 
+        unfolding upd_fi_mu_state.simps state LLL_impl_inv.simps
+      proof (intro conjI)
+        show "list_repr i (update_i f (fs'' ! i)) (map ((!) fs'') [0..<m])" 
+          using update_i[OF list_repr(1), unfolded length_map, OF ii] unfolding repr_id[symmetric] .
+        show "d_repr ds fs''" unfolding to_d_repr[OF impl Linv state, unfolded d_repr_def] d_repr_def
+          by (rule iarray_of_fun_cong, subst step(6), auto)
+        {
+          fix ii
+          assume ii: "ii < m" "ii \<noteq> i" 
+          hence "IArray.sub (IArray.of_fun (\<lambda>i. IArray.of_fun (?mu fs i) (Suc i)) m) ii
+            = IArray.of_fun (?mu fs ii) (Suc ii)" by auto
+          also have "\<dots> = IArray.of_fun (?mu fs'' ii) (Suc ii)" 
+          proof (rule iarray_of_fun_cong, goal_cases)
+            case (1 j)
+            with ii have j: "Suc j \<le> m" by auto
+            show ?case by (subst step(6)[OF j], subst step(5), insert 1 ii, auto)
+          qed
+          finally have "IArray.sub (IArray.of_fun (\<lambda>i. IArray.of_fun (?mu fs i) (Suc i)) m) ii 
+             = IArray.of_fun (?mu fs'' ii) (Suc ii)" by auto
+        } note ii = this
+        show "mu_repr (iarray_update mu i (IArray.of_fun (?mu fs'' i) i)) fs''" 
+          unfolding to_mu_repr[OF impl Linv state, unfolded mu_repr_def] iarray_update_def mu_repr_def 
+           iarray_length_of_fun
+          by (rule iarray_of_fun_cong, insert ii, auto)
+      qed
+    qed (insert i j, auto)
+  qed
+qed
+
+lemma basis_reduction_add_rows: assumes
+     impl: "LLL_impl_inv state i fs" 
+  and inv: "LLL_invariant upw i fs" 
+  and res: "basis_reduction_add_rows upw i state = state'" 
+  and i: "i < m" 
+  and fs': "fs' = fs_state state'" 
+shows 
+  "LLL_impl_inv state' i fs'" 
+  "LLL_invariant False i fs'" 
+  "LLL_measure i fs' = LLL_measure i fs" 
+proof (atomize(full), goal_cases)
+  case 1
+  obtain f mu ds where state: "state = (f,mu,ds)" by (cases state, auto)
+  note def = basis_reduction_add_rows_def
+  show ?case
+  proof (cases upw)
+    case False
+    from LLL_invD[OF inv] have len: "length fs = m" by auto
+    from fs_state[OF impl inv state len] have "fs_state state = fs" by auto
+    with assms False show ?thesis by (auto simp: def)
+  next
+    case True
+    with inv have "LLL_invariant True i fs" by auto
+    note start = this \<mu>_small_row_refl[of i fs]
+    have id: "small_fs_state state = map (\<lambda> i. fs ! i) (rev [0..<i])"
+      unfolding state using to_list_repr[OF impl inv state] i
+      unfolding list_repr_def by (auto intro!: nth_equalityI simp: nth_rev min_def)
+    from i have mm: "[0..<m] = [0 ..< i] @ [i] @ [Suc i ..< m]"
+      by (intro nth_equalityI, auto simp: nth_append nth_Cons split: nat.splits)
+    from res[unfolded def] True 
+    have "basis_reduction_add_rows_loop state i i (small_fs_state state) = state'" by auto
+    from basis_reduction_add_rows_loop[OF impl start(1-2) this[unfolded id] le_refl i fs']
+    show ?thesis by auto
+  qed
+qed
+
+lemma basis_reduction_swap: assumes 
+  impl: "LLL_impl_inv state i fs" 
+  and inv: "LLL_invariant False i fs" 
+  and res: "basis_reduction_swap m i state = (upw',i',state')" 
+  and cond: "sq_norm (gso fs (i - 1)) > \<alpha> * sq_norm (gso fs i)" 
+  and i: "i < m" and i0: "i \<noteq> 0" 
+  and fs': "fs' = fs_state state'" 
+shows 
+  "LLL_impl_inv state' i' fs'" (is ?g1)
+  "LLL_invariant upw' i' fs'" (is ?g2)
+  "LLL_measure i' fs' < LLL_measure i fs" (is ?g3)
+proof -
+  from i i0 have ii: "i - 1 < i" and le_m: "i - 1 \<le> m" "i \<le> m" "Suc i \<le> m" by auto
+  obtain f mu ds where state: "state = (f,mu,ds)" by (cases state, auto)
+  note dmu_ij_state = dmu_ij_state[OF impl inv state]
+  note d_state = d_state[OF impl inv state]
+  note res = res[unfolded basis_reduction_swap_def Let_def split state, folded state,
+    unfolded fi_state[OF impl inv state i] fim1_state[OF impl inv state i i0]] 
+  note state_id = dmu_ij_state[OF ii i] 
+  note d_state_i = d_state[OF le_m(1)] d_state[OF le_m(2)] d_state[OF le_m(3)]
+  from LLL_invD[OF inv] have len: "length fs = m" by auto
+  from fs_state[OF impl inv state len] have fs: "fs_state state = fs" by auto
+  obtain fs'' where fs'': "fs[i := fs ! (i - 1), i - 1 := fs ! i] = fs''" by auto
+  let ?r = rat_of_int
+  let ?n = "\<lambda> i. sq_norm (gso fs i)" 
+  let ?n' = "\<lambda> i. sq_norm (gso fs'' i)" 
+  let ?d = "d fs" 
+  let ?d' = "d fs''" 
+  let ?dn = "\<lambda> i. ?r (?d i * ?d i) * ?n i" 
+  let ?dn' = "\<lambda> i. ?r (?d' i * ?d' i) * ?n' i" 
+  let ?idn = "\<lambda> i. int_of_rat (?dn i)" 
+  let ?idn' = "\<lambda> i. int_of_rat (?dn' i)" 
+  let ?mu = "\<mu> fs" 
+  let ?mu' = "\<mu> fs''" 
+  let ?dmu = "\<lambda> i j. ?r (?d (Suc j)) * ?mu i j" 
+  let ?dmu' = "\<lambda> i j. ?r (?d' (Suc j)) * ?mu' i j" 
+  let ?dmus = "dmu_ij_state state" 
+  let ?ds = "d_state state" 
+  let ?idmu = "\<lambda> i j. int_of_rat (?dmu i j)" 
+  let ?idmu' = "\<lambda> i j. int_of_rat (?dmu' i j)" 
+  let ?x = "?n (i - 1)" 
+  let ?y = "\<alpha> * ?n i" 
+  let ?dd = "?n (i - 1) / ?n' (i - 1)" 
+  let ?mui = "?mu i (i - 1)" 
+  let ?mui' = "?mu' i (i - 1)" 
+  note swap = basis_reduction_swap[OF inv i i0 cond refl, unfolded fs'']
+  note inv' = LLL_invD[OF inv]
+  have nim1: "?n i + square_rat (?mu i (i - 1)) * ?n (i - 1) = 
+    ?n' (i - 1)" by (subst swap(4), insert i, auto)
+  have ni: "?n i * (?n (i - 1) / ?n' (i - 1)) = ?n' i"
+    by (subst swap(4)[of i], insert i i0, auto)
+  have mu': "?mu i (i - 1) * (?n (i - 1) / ?n' (i - 1)) = ?mu' i (i - 1)"
+    by (subst swap(5), insert i i0, auto)
+  have fi: "fs ! (i - 1) = fs'' ! i" "fs ! i = fs'' ! (i - 1)" 
+    unfolding fs''[symmetric] using inv'(7) i i0 by auto
+  from res have upw': "upw' = False" "i' = i - 1" by auto
+  let ?dmu_repr' = "swap_mu m mu i (?dmus i (i - 1)) (?d (i - 1)) (?d i) (?d (Suc i))" 
+  let ?d'i = "(?d (Suc i) * ?d (i - 1) + ?dmus i (i - 1) * ?dmus i (i - 1)) div (?d i)" 
+  from res[unfolded mu' nim1 ni, unfolded fi d_state_i] 
+  have res: "upw' = False" "i' = i - 1" 
+    "state' = (dec_i (update_im1 (update_i f (fs'' ! i)) (fs'' ! (i - 1))), 
+       ?dmu_repr', iarray_update ds i ?d'i)" by auto 
+  from i have ii: "i < length [0..<m]" and im1: "i - 1 < m" by auto
+  note list_repr = to_list_repr[OF impl inv state]
+  from dec_i[OF update_im1[OF update_i[OF list_repr(1)]], unfolded length_map, OF ii i0 i0]
+  have 
+    "list_repr (i - 1) (dec_i (update_im1 (update_i f (fs'' ! i)) (fs'' ! (i - 1)))) (map ((!) fs) [0..<m][i := (fs'' ! i), 
+       i - 1 := (fs'' ! (i - 1))])" (is "list_repr _ ?fr ?xs") .
+  also have "?xs = map ((!) fs'') [0..<m]" unfolding fs''[symmetric]
+    by (intro nth_equalityI, insert i i0 len, auto simp: nth_append, rename_tac ii, case_tac "ii \<in> {i-1,i}", auto)
+  finally have f_repr: "list_repr (i - 1) ?fr (map ((!) fs'') [0..<m])" .    
+  have rat': "ii < m \<Longrightarrow> j < ii \<Longrightarrow> ?r (?idmu' ii j) = ?dmu' ii j" for ii j 
+     using LLL_mu_d_Z[OF swap(1), of j ii] by simp
+  have rat: "ii < m \<Longrightarrow> j < ii \<Longrightarrow> ?dmu ii j = ?r (?dmus ii j)"
+     "ii < m \<Longrightarrow> j < ii \<Longrightarrow> ?idmu ii j = ?dmus ii j" for ii j 
+    using LLL_mu_d_Z[OF inv, of j ii]
+    using dmu_ij_state[of j ii, symmetric] by auto
+  from i0 have sim1: "Suc (i - 1) = i" by simp
+  from LLL_d_Suc[OF inv im1, unfolded sim1] 
+  have dn_im1: "?dn (i - 1) = ?r (?d i) * ?r (?d (i - 1))" by simp
+
+  note pos = Gramian_determinant[OF inv le_refl] 
+  from pos(2) have "?r (gs.Gramian_determinant fs m) \<noteq> 0" by auto
+  from this[unfolded pos(1)] have nzero: "ii < m \<Longrightarrow> ?n ii \<noteq> 0" for ii by auto
+  note pos = Gramian_determinant[OF swap(1) le_refl] 
+  from pos(2) have "?r (gs.Gramian_determinant fs'' m) \<noteq> 0" by auto
+  from this[unfolded pos(1)] have nzero': "ii < m \<Longrightarrow> ?n' ii \<noteq> 0" for ii by auto
+  have dzero: "ii \<le> m \<Longrightarrow> ?d ii \<noteq> 0" for ii using LLL_d_pos[OF inv, of ii] by auto
+  have dzero': "ii \<le> m \<Longrightarrow> ?d' ii \<noteq> 0" for ii using LLL_d_pos[OF swap(1), of ii] by auto
+
+  {
+    define start where "start = ?dmu' i (i - 1)" 
+    have "start = (?n' (i - 1) / ?n (i - 1) * ?r (?d i)) * ?mu' i (i - 1)" 
+      using start_def swap(6)[of i] i i0 by simp
+    also have "?mu' i (i - 1) = ?mu i (i - 1) * (?n (i - 1) / ?n' (i - 1))" 
+      using mu' by simp
+    also have "(?n' (i - 1) / ?n (i - 1) * ?r (?d i)) * \<dots> = ?r (?d i) * ?mu i (i - 1)" 
+      using nzero[OF im1] nzero'[OF im1] by simp
+    also have "\<dots> = ?dmu i (i - 1)" using i0 by simp
+    finally have "?dmu' i (i - 1) = ?dmu i (i - 1)" unfolding start_def .
+  } note dmu_i_im1 = this
+  have mu_ij: "ii < m \<Longrightarrow> j < ii \<Longrightarrow> ?idmu ii j = ?dmus ii j" for ii j
+    using dmu_ij_state[symmetric, of j ii]  by auto
+  { (* d updates *)
+    fix j
+    assume j: "j \<le> m" 
+    define start where "start = ?d' j" 
+    {
+      assume jj: "j \<noteq> i" 
+      have "?r start = ?r (?d' j)" unfolding start_def ..
+      also have "?r (?d' j) = ?r (?d j)" 
+        by (subst swap(6), insert j jj, auto)
+      finally have "start = ?d j" by simp
+    } note d_j = this 
+    {
+      assume jj: "j = i"  
+      have "?r start = ?r (?d' i)" unfolding start_def unfolding jj by simp
+      also have "\<dots> = ?n' (i - 1) / ?n (i - 1) * ?r (?d i)" 
+        by (subst swap(6), insert i, auto)
+      also have "?n' (i - 1) = (?r (?d i) / ?r (?d i)) * (?r (?d i) / ?r (?d i)) 
+          * (?n i  + ?mu i (i - 1) * ?mu i (i - 1) * ?n (i - 1))" 
+        by (subst swap(4)[OF im1], insert dzero[of i], insert i, simp)
+      also have "?n (i - 1) = ?r (?d i) / ?r (?d (i - 1))" 
+        unfolding LLL_d_Suc[OF inv im1, unfolded sim1] using dzero[of "i - 1"] i0 i by simp
+      finally have "?r start = 
+          ((?r (?d i) * ?n i) * ?r (?d (i - 1)) + ?dmu i (i - 1) * ?dmu i (i - 1)) 
+          / (?r (?d i))" 
+        using i0 dzero[of i] i dzero[of "i - 1"]
+        by (simp add: ring_distribs)
+      also have "?r (?d i) * ?n i = ?r (?d (Suc i))" 
+        unfolding LLL_d_Suc[OF inv i] by simp
+      also have "?dmu i (i - 1) = ?r (?dmus i (i - 1))" by (rule rat, insert i i0, auto)
+      finally have "?r start = (?r (?d (Suc i) * ?d (i - 1) + ?dmus i (i - 1) * ?dmus i (i - 1)))
+          / (?r (?d i))" by simp
+      from division_to_div[OF this]
+      have "start = ?d'i" .
+    } note d_i = this
+    from d_j d_i have "?d' j = (if j = i then ?d'i else ?d j)" unfolding start_def by auto
+  } note d_update = this
+  have "length fs'' = m" 
+    using fs'' inv'(7) by auto
+  hence fs_id: "fs' = fs''" unfolding fs' res fs_state.simps using of_list_repr[OF f_repr] 
+    by (intro nth_equalityI, auto simp: o_def)
+  from to_mu_repr[OF impl inv state] have mu: "mu_repr mu fs" by auto
+  from to_d_repr[OF impl inv state] have d_repr: "d_repr ds fs" by auto
+  note mu_def = mu[unfolded mu_repr_def]
+  show ?g1 unfolding fs_id LLL_impl_inv.simps res
+  proof (intro conjI f_repr)
+    show "d_repr (iarray_update ds i ?d'i) fs''" 
+      unfolding d_repr[unfolded d_repr_def] iarray_update_def d_repr_def iarray_length_of_fun
+      by (rule iarray_of_fun_cong, subst d_update, auto simp: nth_append intro: arg_cong)
+    show "mu_repr ?dmu_repr' fs''" unfolding mu_repr_def swap_mu_def Let_def
+    proof (rule iarray_of_fun_cong, goal_cases)
+      case ii: (1 ii) 
+      show ?case
+      proof (cases "ii < i - 1")
+        case small: True
+        hence id: "(ii = i) = False" "(ii = i - 1) = False" "(i < ii) = False" "(ii < i - 1) = True" by auto
+        have mu: "IArray.sub mu ii = IArray.of_fun (\<lambda>j. int_of_rat (?r (d fs (Suc j)) * \<mu> fs ii j)) ii" 
+          using ii unfolding mu_def by auto
+        show ?thesis unfolding id if_True if_False mu
+        proof (rule iarray_of_fun_cong, goal_cases)
+          case j: (1 j)
+          with ii swap(5)[of ii j, unfolded id if_False] swap(6)[of "Suc j"] i i0 small show ?case by auto
+        qed
+      next
+        case False
+        hence iFalse: "(ii < i - 1) = False" by simp
+        show ?thesis unfolding iFalse if_False if_distrib[of "\<lambda> f. IArray.of_fun f ii", symmetric]
+          dmu_ij_state.simps[of f mu ds, folded state, symmetric] 
+        proof (rule iarray_of_fun_cong, goal_cases)
+          case j: (1 j)
+          let ?start = "?idmu' ii j" 
+          define start where "start = ?start" 
+          from j ii have sj: "Suc j \<le> m" by auto
+          note mu_ij[OF ii j]
+          note rat'[OF ii j]
+          note rat_ii_j = rat[OF ii j]
+          note swaps = swap(5)[OF ii j] swap(6)[OF sj]
+          from False consider (I) "ii = i" "j = i - 1" | (Is) "ii = i" "j \<noteq> i - 1" | 
+            (Im1) "ii = i - 1" | (large) "ii > i" by linarith
+          thus ?case
+          proof cases
+            case iii: Is
+            with j have j: "j < i - 1" by auto
+            have "?start = ?idmu (i - 1) j" unfolding swaps using iii ii i j i0 by auto
+            also have "\<dots> = ?dmus (i - 1) j" by (subst mu_ij, insert iii i j , auto)
+            finally show ?thesis using iii j by auto
+          next
+            case iii: I
+            with j i0 have j: "j = i - 1" "Suc j = i" by auto
+            have "?r (?start) = ?dmu' ii j" by fact
+            also have "\<dots> = ?dmu i (i - 1)" unfolding iii j using dmu_i_im1 i0 by simp 
+            also have "\<dots> = ?dmu ii j" unfolding j iii ..
+            also have "\<dots> = ?r (?idmu ii j)" using rat_ii_j by simp
+            finally have "?r ?start = ?r (?idmu ii j)" .
+            hence "?start = ?idmu ii j" by simp
+            also have "\<dots> = ?dmus ii j" by fact
+            finally have "?start = ?dmus ii j" .
+            thus ?thesis using iii by auto
+          next
+            case iii: Im1
+            have "?start = ?idmu i j" unfolding swaps using iii ii i j i0 by auto
+            also have "\<dots> = ?dmus i j" by (subst mu_ij, insert iii i j , auto)
+            finally have id: "?start = ?dmus i j" .
+            from iii have id': "(i < ii) = False" "(ii = i) = False" using i0 by auto
+            show ?thesis unfolding id id' if_False ..
+          next
+            case iii: large
+            hence id': "(i < ii) = True" by auto
+            consider (jj) "j \<noteq> i - 1" "j \<noteq> i" | (ji) "j = i" | (jim1) "j = i - 1" by linarith
+            thus ?thesis 
+            proof cases
+              case jj
+              have "?start = ?idmu ii j" unfolding swaps using iii ii i jj i0 by auto
+              also have "\<dots> = ?dmus ii j" by fact
+              finally have id: "?start = ?dmus ii j" .
+              show ?thesis unfolding id id' if_True using jj by auto
+            next
+              case ji
+              have "?r start = ?dmu' ii j" unfolding start_def by fact
+              also have "?r (?d' (Suc j)) = ?r (?d (Suc i))" unfolding swaps unfolding ji by simp 
+              also have "?mu' ii j = ?mu ii (i - 1) - ?mu i (i - 1) * ?mu ii i" 
+                unfolding swaps unfolding ji using i0 iii by auto
+              also have "?r (?d (Suc i)) * \<dots> = ?r (?d (Suc i)) * ?r (?d i) / ?r (?d i) * \<dots>" 
+                using dzero[of i] i by auto
+              also have "\<dots> =  
+                (?r (?d (Suc i)) * ?dmu ii (i - 1) - ?dmu i (i - 1) * ?dmu ii i) / ?r (?d i)" 
+                using i0 by (simp add: field_simps)
+              also have "\<dots> = 
+                (?r (?d (Suc i)) * ?r (?dmus ii (i - 1)) - ?r (?dmus i (i - 1)) * ?r (?dmus ii i)) / ?r (?d i)" 
+                by (subst (1 2 3) rat, insert i i0 ii iii, auto)
+              also have "\<dots> = ?r (?d (Suc i) * ?dmus ii (i - 1) - ?dmus i (i - 1) * ?dmus ii i) / ?r (?d i)" 
+                (is "_ = of_int ?x / _")
+                by simp
+              finally have "?r start = ?r ?x / ?r (?d i)" .
+              from division_to_div[OF this]
+              have id: "?start = (?d (Suc i) * ?dmus ii (i - 1) - ?dmus i (i - 1) * ?dmus ii i) div ?d i" 
+                unfolding start_def .
+              show ?thesis unfolding id' id if_True using ji by auto
+            next
+              case jim1
+              hence id'': "(j = i - 1) = True" "(j = i) = False" using i0 by auto
+              have "?r (start) = ?dmu' ii j" unfolding start_def by fact
+              also have "?mu' ii j = ?mu ii (i - 1) * ?mu' i (i - 1) +
+                                 ?mu ii i * ?n i / ?n' (i - 1)" (is "_ = ?x1 + ?x2")
+                unfolding swaps unfolding jim1 using i0 iii by auto
+              also have "?r (?d' (Suc j)) * (?x1 + ?x2)
+                  = ?r (?d' (Suc j)) * ?x1 + ?r (?d' (Suc j)) * ?x2" by (simp add: ring_distribs)
+              also have "?r (?d' (Suc j)) * ?x1 = ?dmu' i (i - 1) * (?r (?d i) * ?mu ii (i - 1))
+                / ?r (?d i)"
+                unfolding jim1 using i0 dzero[of i] i by simp
+              also have "?dmu' i (i - 1) = ?dmu i (i - 1)" by fact
+              also have "?r (?d i) * ?mu ii (i - 1) = ?dmu ii (i - 1)" using i0 by simp
+              also have "?r (?d' (Suc j)) = ?n' (i - 1) * ?r (?d i) / ?n (i - 1)" 
+                unfolding swaps unfolding jim1 using i0 i by simp 
+              also have "\<dots> * ?x2 = (?n i * ?r (?d i)) / ?n (i - 1) * ?mu ii i" 
+                using i0 nzero'[of "i - 1"] i by simp
+              also have "?n i * ?r (?d i) = ?r (?d (Suc i))" unfolding LLL_d_Suc[OF inv i] ..
+              also have "?r (?d (Suc i)) / ?n (i - 1) * ?mu ii i = ?dmu ii i / ?n (i - 1)" by simp
+              also have "\<dots> = ?dmu ii i * ?r (?d (i - 1) * ?d (i - 1)) / ?dn (i - 1)" 
+                using dzero[of "i - 1"] i by simp
+              finally have "?r start = (?dmu i (i - 1) * ?dmu ii j * ?dn (i - 1) + 
+                 ?dmu ii i * (?r (?d (i - 1) * ?d (i - 1) * ?d i))) / (?r (?d i) * ?dn (i - 1))"
+                unfolding add_divide_distrib of_int_mult jim1
+                using dzero[of "i - 1"] nzero[of "i - 1"] i dzero[of i] by auto
+              also have "\<dots> = (?r (?dmus i (i - 1)) * ?r (?dmus ii j) * (?r (?d i) * ?r (?d (i - 1))) + 
+                 ?r (?dmus ii i) * (?r (?d (i - 1) * ?d (i - 1) * ?d i))) / (?r (?d i) * (?r (?d i) * ?r (?d (i - 1))))" 
+                unfolding dn_im1 
+                by (subst (1 2 3) rat, insert i ii iii i0 j, auto)
+              also have "\<dots> = (?r (?dmus i (i - 1)) * ?r (?dmus ii j) + ?r (?dmus ii i) * ?r (?d (i - 1))) 
+                  / ?r (?d i)" 
+                unfolding of_int_mult using dzero[of i] dzero[of "i - 1"] i i0 by (auto simp: field_simps)
+              also have "\<dots> = ?r (?dmus i (i - 1) * ?dmus ii j + ?dmus ii i * ?d (i - 1)) / ?r (?d i)" 
+                (is "_ = of_int ?x / _" )
+                by simp
+              finally have "?r start = ?r ?x / ?r (?d i)" .
+              from division_to_div[OF this]
+              have id: "?start = (?dmus i (i - 1) * ?dmus ii j + ?dmus ii i * ?d (i - 1)) div (?d i)" 
+                unfolding start_def .
+              show ?thesis unfolding id id' id'' if_True if_False ..
+            qed
+          qed
+        qed
+      qed
+    qed
+  qed
+  from swap(1-2) fs_id show ?g2 ?g3 using res by auto
+qed
+
+lemma basis_reduction_step: assumes 
+  impl: "LLL_impl_inv state i fs" 
+  and inv: "LLL_invariant upw i fs" 
+  and res: "basis_reduction_step \<alpha> m upw i state = (upw',i',state')" 
+  and i: "i < m" 
+  and fs': "fs' = fs_state state'" 
+shows 
+  "LLL_impl_inv state' i' fs'" 
+  "LLL_invariant upw' i' fs'" 
+  "LLL_measure i' fs' < LLL_measure i fs" 
+proof (atomize(full), goal_cases)
+  case 1
+  obtain f mu ds where state: "state = (f,mu,ds)" by (cases state, auto)
+  note def = basis_reduction_step_def
+  from LLL_invD[OF inv] have len: "length fs = m" by auto
+  from fs_state[OF impl inv state len] have fs: "fs_state state = fs" by auto
+  show ?case
+  proof (cases "i = 0")
+    case True
+    from LLL_state_inc_state[OF impl inv state i] i
+      assms increase_i[OF inv i True] True 
+      res fs' fs
+    show ?thesis by (auto simp: def)
+  next
+    case False
+    hence id: "(i = 0) = False" by auto
+    obtain state'' where state'': "basis_reduction_add_rows upw i state = state''" by auto
+    define fs'' where fs'': "fs'' = fs_state state''" 
+    obtain f mu ds where state: "state'' = (f,mu,ds)" by (cases state'', auto)
+    from basis_reduction_add_rows[OF impl inv state'' i fs'']
+    have inv: "LLL_invariant False i fs''"
+      and meas: "LLL_measure i fs = LLL_measure i fs''" 
+      and impl: "LLL_impl_inv state'' i fs''" by auto
+    obtain num denom where quot: "quotient_of \<alpha> = (num,denom)" by force
+    note d_state = d_state[OF impl inv state]
+    from i have le: "i - 1 \<le> m" " i \<le> m" "Suc i \<le> m" by auto
+    note d_state = d_state[OF le(1)] d_state[OF le(2)] d_state[OF le(3)]
+    note res = res[unfolded def id if_False Let_def state'' quot split d_state] 
+    note pos = LLL_d_pos[OF inv le(1)] LLL_d_pos[OF inv le(2)] quotient_of_denom_pos[OF quot]
+    from False have sim1: "Suc (i - 1) = i" by simp
+    let ?r = "rat_of_int" 
+    let ?x = "sq_norm (gso fs'' (i - 1))" 
+    let ?y = "\<alpha> * sq_norm (gso fs'' i)" 
+    have "(d fs'' i * d fs'' i * denom \<le> num * d fs'' (i - 1) * d fs'' (Suc i))
+      = (?r (d fs'' i * d fs'' i * denom) \<le> ?r (num * d fs'' (i - 1) * d fs'' (Suc i)))" (is "?cond = _") by presburger
+    also have "\<dots> = (?r (d fs'' i) * ?r (d fs'' i) * ?r denom \<le> ?r num * ?r (d fs'' (i - 1)) * ?r (d fs'' (Suc i)))" by simp
+    also have "\<dots> = (?r (d fs'' i) * ?r (d fs'' i) \<le> \<alpha> * ?r (d fs'' (i - 1)) * ?r (d fs'' (Suc i)))" 
+      using pos unfolding quotient_of_div[OF quot] by (auto simp: field_simps)
+    also have "\<dots> = (?r (d fs'' i) / ?r (d fs'' (i - 1)) \<le> \<alpha> * (?r (d fs'' (Suc i)) / ?r (d fs'' i)))" 
+      using pos by (auto simp: field_simps)
+    also have "?r (d fs'' i) / ?r (d fs'' (i - 1)) = ?x" using LLL_d_Suc[OF inv, of "i - 1"] pos i False
+      by (auto simp: field_simps)
+    also have "\<alpha> * (?r (d fs'' (Suc i)) / ?r (d fs'' i)) = ?y" using LLL_d_Suc[OF inv i] pos i False
+      by (auto simp: field_simps)
+    finally have "?cond = (?x \<le> ?y)" .
+    note res = res[unfolded this]
+    show ?thesis
+    proof (cases "?x \<le> ?y")
+      case True
+      from increase_i[OF inv i _ True] True res meas LLL_state_inc_state[OF impl inv state i] fs' fs''
+      show ?thesis by auto
+    next
+      case gt: False
+      hence gt: "?x > ?y" and id: "(?x \<le> ?y) = False" by auto
+      from res[unfolded id if_False] have "basis_reduction_swap m i state'' = (upw', i', state')" by auto
+      from basis_reduction_swap[OF impl inv this gt i False fs'] show ?thesis using meas by auto
+    qed
+  qed
+qed
+
+lemma basis_reduction_main: assumes 
+  impl: "LLL_impl_inv state i fs" 
+  and inv: "LLL_invariant upw i fs" 
+  and res: "basis_reduction_main \<alpha> m upw i state = state'" 
+  and fs': "fs' = fs_state state'" 
+shows "LLL_invariant True m fs'" 
+      "LLL_impl_inv state' m fs'" 
+proof (atomize(full), insert assms(1-3), induct "LLL_measure i fs" arbitrary: i fs upw state rule: less_induct)
+  case (less i fs upw)
+  have id: "LLL_invariant upw i fs = True" using less by auto
+  note res = less(4)[unfolded basis_reduction_main.simps[of _ _ upw]]
+  note inv = less(3)
+  note impl = less(2)
+  note IH = less(1)
+  show ?case
+  proof (cases "i < m")
+    case i: True
+    obtain i'' state'' upw'' where step: "basis_reduction_step \<alpha> m upw i state = (upw'',i'',state'')" 
+      (is "?step = _") by (cases ?step, auto)
+    with res i have res: "basis_reduction_main \<alpha> m upw'' i'' state'' = state'" by auto
+    note main = basis_reduction_step[OF impl inv step i refl]
+    from IH[OF main(3,1,2) res]
+    show ?thesis by auto
+  next
+    case False
+    from LLL_invD[OF inv] have len: "length fs = m" by auto
+    obtain f mu ds where state: "state = (f,mu,ds)" by (cases state, auto)
+    from fs_state[OF impl inv state len] have fs: "fs_state state = fs" by auto
+    from False LLL_invD[OF inv] have i: "i = m" upw by auto
+    with False res inv impl fs show ?thesis by (auto simp: fs')
+  qed
+qed
+
+lemma initial_state: "LLL_impl_inv (initial_state n m fs_init) 0 fs_init" 
+proof -
+  note conn = gs.main_connect[OF lin_dep, unfolded length_map, OF len refl]
+  have id: "gram_schmidt n (RAT fs_init) = map (gso fs_init) [0..<m]" 
+    using conn by auto
+  have f_repr: "list_repr 0 ([], fs_init) (map ((!) fs_init) [0..<m])" 
+    unfolding list_repr_def by (simp, intro nth_equalityI, auto simp: len)
+  from fs_init have Rn: "set (RAT fs_init) \<subseteq> Rn" by auto
+  have 1: "1 = d fs_init 0" unfolding d_def gs.Gramian_determinant_def gs.Gramian_matrix_def Let_def
+    by (simp add: times_mat_def)
+  define j where "j = m" 
+  have jm: "j \<le> m" unfolding j_def by auto
+  have 0: "0 = m - j" unfolding j_def by auto
+  have d_repr: "d_repr (IArray (norms_to_ds 1 (map (\<lambda>j. \<parallel>gs.gso (map of_int_hom.vec_hom fs_init) j\<parallel>\<^sup>2) [0..<m]))) fs_init" 
+    unfolding d_repr_def IArray.of_fun_def 1 0
+  proof (rule arg_cong[of _ _ IArray], insert jm, induct j)
+    case (Suc j)
+    hence small: "m - Suc j < m" and [simp]: "Suc (m - Suc j) = m - j" by auto
+    have id0: "snd (gs.main (RAT fs_init)) ! (m - Suc j) = gso fs_init (m - Suc j)" 
+      unfolding conn using Suc by simp 
+    from Suc(2-) have id1: "[m - Suc j..<m] = (m - Suc j) # [m - j ..<m]"
+      "[m - Suc j..<Suc m] = (m - Suc j) # [m - j ..< Suc m]"
+      by (auto simp add: Suc_diff_Suc Suc_le_lessD upt_conv_Cons)
+    {
+      fix j
+      assume j: "j \<le> m" 
+      have "gs.Gramian_determinant (RAT fs_init) j = of_int (d fs_init j)" 
+        unfolding d_def
+        by (rule of_int_Gramian_determinant, insert len fs_init j, auto simp: set_conv_nth)
+    } note conv = this
+    from Suc have le: "m - (Suc j) \<le> m" by auto
+    note nzero = 
+      gs.Gramian_determinant(2)[OF lin_dep, unfolded length_map, OF len refl le, unfolded conv[OF le]]
+    have id': "(int_of_rat (rat_of_int (d fs_init (m - Suc j)) * \<parallel>gso fs_init (m - Suc j)\<parallel>\<^sup>2))
+        = d fs_init (m - j)" 
+      by (rule int_via_rat_eqI, 
+      unfold gs.Gramian_determinant_div[OF lin_dep, unfolded length_map, OF len refl small, symmetric, unfolded id0],
+      subst (1 2) conv, insert Suc(2-) nzero, auto)      
+    show ?case unfolding id1 list.simps norms_to_ds.simps int_times_rat_def id'
+      by (intro conjI[OF refl Suc(1)], insert Suc(2-), auto)
+  qed simp
+  show ?thesis unfolding initial_state_def Let_def LLL_impl_inv.simps gram_schmidt_triv id
+    norms_mus_rat_norms_mus 
+    gs.norms_mus[OF Rn, unfolded length_map len, OF gs.mn[OF lin_dep, unfolded length_map, OF len refl]]
+    fst_conv snd_conv split
+    by (intro conjI f_repr d_repr, unfold d_repr[unfolded d_repr_def] int_times_rat_def mu_repr_def,
+      intro iarray_of_fun_cong, auto simp: nth_append)
+qed
+
+lemma basis_reduction: assumes res: "basis_reduction \<alpha> n fs_init = state" 
+  and fs: "fs = fs_state state" 
+shows "LLL_invariant True m fs" 
+  "LLL_impl_inv state m fs" 
+  using basis_reduction_main[OF initial_state LLL_inv_initial_state res[unfolded basis_reduction_def len] fs]
+  by auto
+
+lemma reduce_basis: assumes res: "reduce_basis \<alpha> fs_init = fs" 
+  shows "gs.reduced \<alpha> m (map (gso fs) [0..<m]) (\<mu> fs)" "LLL_invariant True m fs" 
+proof -
+  show "LLL_invariant True m fs" 
+  proof (cases fs_init)
+    case (Cons f)
+    from fs_init[unfolded Cons] have "dim_vec f = n" by auto
+    from res[unfolded reduce_basis_def Cons list.simps this, folded Cons]
+    have "fs_state (basis_reduction \<alpha> n fs_init) = fs" by auto
+    from basis_reduction(1)[OF refl refl, unfolded this] show "LLL_invariant True m fs" .
+  next
+    case Nil
+    with len have m0: "m = 0" by auto
+    from Nil res have fs: "fs = fs_init" unfolding reduce_basis_def by auto
+    show "LLL_invariant True m fs" unfolding fs LLL_invariant_def L_def gs.reduced_def gs.weakly_reduced_def 
+      using lin_dep unfolding m0 Nil by auto
+  qed
+  thus "gs.reduced \<alpha> m (map (gso fs) [0..<m]) (\<mu> fs)" by (rule LLL_inv_m_imp_reduced)
+qed
+
+lemma short_vector: assumes res: "short_vector \<alpha> fs_init = v"
+  and m0: "m \<noteq> 0"
+shows "v \<in> carrier_vec n"
+  "v \<in> L - {0\<^sub>v n}"  
+  "h \<in> L - {0\<^sub>v n} \<Longrightarrow> rat_of_int (sq_norm v) \<le> \<alpha> ^ (m - 1) * rat_of_int (sq_norm h)" 
+  "v \<noteq> 0\<^sub>v j" 
+  using basis_reduction_short_vector[OF reduce_basis(2)[OF refl] res[symmetric, unfolded short_vector_def] m0] 
+  by blast+
+
+end
+end
